Update goose and ownership lectures

go/heap/binary_search.go
@@ -1,0 +1,24 @@
+package heap
+
+// BinarySearch looks for needle in the sorted list s. It returns (index, found)
+// where if found = false, needle is not present in s, and if found = true, s[index]
+// == needle.
+//
+// If needle appears multiple times in s, no guarantees are made about which of
+// those indices is returned.
+func BinarySearch(s []uint64, needle uint64) (uint64, bool) {
+	var i = uint64(0)
+	var j = uint64(len(s))
+	for i < j {
+		mid := i + (j-i)/2
+		if s[mid] < needle {
+			i = mid + 1
+		} else {
+			j = mid
+		}
+	}
+	if i < uint64(len(s)) {
+		return i, s[i] == needle
+	}
+	return i, false
+}
