go/heap/binary_search_test.go
@@ -1,0 +1,28 @@
+package heap
+
+import (
+	"testing"
+
+	"github.com/stretchr/testify/assert"
+)
+
+func TestBinarySearch(t *testing.T) {
+	assert := assert.New(t)
+
+	s := []uint64{1, 3, 4, 5}
+	var i uint64
+	var ok bool
+	i, ok = BinarySearch(s, 2)
+	assert.False(ok)
+
+	i, ok = BinarySearch(s, 1)
+	assert.Equal(uint64(0), i)
+	assert.True(ok)
+
+	i, ok = BinarySearch(s, 5)
+	assert.Equal(uint64(3), i)
+	assert.True(ok)
+
+	i, ok = BinarySearch(s, 6)
+	assert.False(ok)
+}
