src/sys_verif/program_proof/ownership.v
@@ -307,13 +307,23 @@ You can ignore this whole string of parameters, which are related to Goose suppo
 
 Getting and setting slice elements have reasonable specifications:
 
-::: warning TODO
+|*)
 
-copy these from perennial
+Check wp_SliceGet.
 
-:::
+(*| We got this specification using `Check` rather than copying it from the Perennial source code. Notice that the Hoare triple notation is not used here (I'm not entirely sure why, possibly a bug in the notations). You should still be able to read this specification, if you understood the "continuation-passing style" encoding of Hoare triple used in Iris.
 
-### Appending to a slice
+The one complication with this particular specification is that its precondition requires the caller to pass the value `v0` that is in the slice. `SliceGet` itself requires `i` to be in-bounds (otherwise `s[i]` panics in Go), and `vs !! uint.nat i = Some v0` has the side of enforcing this obligation, and the postcondition then uses the same value `v0`.
+|*)
+
+Check wp_SliceSet.
+
+(*| Storing into a slice requires a proof `is_Some (vs !! uint.nat i)`, which similarly guarantees that `i` is in-bounds, but the original value is not needed. The postcondition uses `<[uint.nat i := v]> vs` which is a Gallina implementation of updating one index of a list (it's notation for the function `insert` from std++).
+
+You may notice that there's an arbitrary `q : dfrac` in the specification for `SliceGet`, while `SliceSet` has `DfracOwn 1`. This difference is no accident and corresponds to the fact that `SliceGet` works even on a _read-only_ slice while `SliceSet` needs to be able to modify the input slice. We'll cover the mechanism with fractions [later on](#read-only).
+|*)
+
+(*| ### Appending to a slice
 
 The capacity of a slice is interesting in the model because it turns out ownership of the capacity is separate from ownership of the elements. Consider the following code, which splits a slice:
 
@@ -359,19 +369,19 @@ What is key to understanding the Go example above is that the Go expression `s[:
 There is one more possibility which is a slight variation on splitting:
 - `own_slice s dq t xs ⊢ own_slice_small (slice_take s dq t (take xs n)) ∗ own_slice (slice_drop s dq t (drop xs n))`. If we start out with ownership of the capacity, we can split ownership and still be able to append to the _second_ part (its capacity is the capacity of the original slice). We can actually derive this from the lower-level fact that `slice_cap s t ⊣⊢ slice_cap (slice_skip s n)` if `n` is in-bounds.
 
+### Exercise: find the theorems above in Perennial
+
+Either using `Search` or by looking at the source code in Perennial, find the theorems above.
+
+The relevant source code is the file `src/goose_lang/lib/slice/typed_slice.v` in Perennial (you can use the submodule copy in your exercises repo).
+
 |*)
 
-(*| ## Maps
+(*| ## Read-only ownership: fractional permissions {#read-only}
 
-## Fractional permissions
+Fractional permissions are an approach to reasoning about read-only access in separation logic.
 
-Covered reasonably well already in [fractional permissions](./program-proofs/fractions.md)
-
-"Fictional separation".
-
-Fractional permission models read-only access.
-
-Discardable fractions.
+This concept is explained as part of the Program Proofs guide in [fractional permissions](./program-proofs/fractions.md).
 
 |*)
 
